src/PartialMonotonicity.v
@@ -2,47 +2,38 @@
 (* Clément Blaudeau - LAMP@EPFL 2021 *)
 (** This file defines the notion of partial monotonicity between stores. The idea behind partial monotonicity is simple: objects that are being initialized (not warm already) can only get "warmer": the number of initialized fields can only increase. Between two stores [σ] and [σ'], it means that all objects in [σ] have more initialized fields in [σ']; it does not states anything about new objects that [σ'] can have. *)
 
-From Celsius Require Export Compatibility Reachability.
+From Celsius Require Export Semantics.
 Require Import ssreflect ssrbool List Psatz Coq.Program.Tactics.
 Import ListNotations.
 Open Scope nat_scope.
 
 (** ** Definitions and notations *)
-Definition initialized_fields σ l (f: list Field) : Prop :=
-  match (getObj σ l) with
-  | Some (C, ω) => ((length f) <= (length ω))
-  | _ => False
-  end.
-
-Global Instance notation_initialized_fields : notation_dash_colon Store Loc (list Field) :=
-  { dash_colon_ := initialized_fields }.
-Global Hint Unfold notation_initialized_fields: notations.
-
 Definition partial_monotonicity σ σ' :=
-  forall l f, (σ ⊨ l : f) -> (σ' ⊨ l : f).
-
+  forall l C ω, getObj σ l = Some(C, ω) -> exists ω', getObj σ' l = Some(C, ω') /\ dom ω <= dom ω'.
 Notation "s ⪯ s'" := (partial_monotonicity s s') (at level 60).
+Definition exact_monotonicity σ σ' :=
+  forall l C ω, getObj σ l = Some(C, ω) -> exists ω', getObj σ' l = Some(C, ω') /\ dom ω = dom ω'.
+Notation "s ⪳ s'" := (exact_monotonicity s s') (at level 60).
 
 Local Hint Unfold partial_monotonicity: pM.
-Local Hint Unfold initialized_fields: pM.
+Local Hint Unfold exact_monotonicity: pM.
 Implicit Type σ: Store.
 
-(** ** Basic results *)
-(** The relation is trivially reflexive *)
+(** ** Basic results on partial monotonicity*)
+(** The relation is trivially reflexive and transitive *)
 Lemma pM_refl: forall σ,
     σ ⪯ σ.
-Proof.
-  auto with pM.
-Qed.
+Proof. eauto with pM. Qed.
 Global Hint Resolve pM_refl: pM.
 
-(** The relation is trivially transitive *)
 Lemma pM_trans : forall σ1 σ2 σ3,
     σ1 ⪯ σ2 ->
     σ2 ⪯ σ3 ->
     σ1 ⪯ σ3.
 Proof.
-  autounfold with notations. eauto with pM.
+  unfold partial_monotonicity; intros.
+  specialize (H l C ω); steps.
+  specialize (H0 l C ω'); steps; eauto with pM lia.
 Qed.
 Global Hint Resolve pM_trans: pM.
 
@@ -55,31 +46,6 @@ Ltac pM_trans :=
 Global Hint Extern 1 => pM_trans: pM.
 
 
-(** Initialized fields are within the domain *)
-Lemma initialized_fields_dom :
-  forall σ l f,
-    (σ ⊨ l : f) -> (l < (dom σ)).
-Proof.
-  autounfold with notations.
-  unfold initialized_fields, getObj.
-  induction σ; destruct l as [| l']; steps; try lia.
-  eapply Le.le_n_S, IHσ; rewrite_any; eauto.
-Qed.
-Global Hint Resolve initialized_fields_dom: pM.
-
-(** Technical result: an object always have 0 or more fields initialized *)
-Lemma initialized_fields_exists :
-  forall σ C ω,
-  exists f, ((C,ω)::σ) ⊨ (dom σ) : f.
-Proof.
-  autounfold with notations pM core.
-  unfold initialized_fields.
-  intros. exists ([]: list Field).
-  induction σ; intros ; simpl ; try lia.
-  destruct σ, a; steps; lia.
-Qed.
-Global Hint Resolve initialized_fields_exists: pM.
-
 (** We have a result on the store sizes *)
 Lemma pM_domains:
   forall σ σ',
@@ -87,9 +53,15 @@ Lemma pM_domains:
 Proof.
   autounfold; unfold partial_monotonicity; intros.
   destruct σ eqn:Σ; simpl; [lia |].
-  destruct o.
-  move : (initialized_fields_exists s c e) => [f Hf].
-  eauto using Lt.lt_le_S with pM.
+  destruct o as [C ω].
+  specialize (H (dom s)).
+  destruct (getObj ((C, ω)::s) (dom s)) eqn: H__e.
+  - destruct o as [D ω'].
+    apply H in H__e; steps.
+    apply getObj_dom in H1; auto.
+  - unfold getObj in H__e.
+    apply nth_error_None in H__e.
+    simpl in H__e; lia.
 Qed.
 Global Hint Resolve pM_domains: pM.
 
@@ -108,6 +80,7 @@ Proof.
     repeat rewrite_any;
     rewrite getObj_update1 || rewrite getObj_update2;
     eauto using getObj_dom.
+  steps. eexists; split; eauto.
 Qed.
 Global Hint Resolve pM_assignment: pM.
 
@@ -115,10 +88,9 @@ Lemma pM_freshness :
   forall σ c ρ,
     σ ⪯ (σ ++ [(c, ρ)]).
 Proof.
-  autounfold with notations pM. unfold getObj.
-  steps;
-    rewrite nth_error_app1 in matched; steps;
-    apply nth_error_Some; steps.
+  autounfold with notations pM. unfold getObj; intros.
+  exists ω; steps.
+  rewrite nth_error_app1; eauto using getObj_dom.
 Qed.
 Global Hint Resolve pM_freshness: pM.
 
@@ -130,14 +102,14 @@ Proof with (eauto with pM updates lia).
   intros.
   induction H using evalP_ind2 with
     (Pl := fun _ σ _ _ _ σ' _ => σ ⪯ σ')
-    (Pin := fun _ _ _ σ σ' _ => σ ⪯ σ');
+    (Pin := fun _ _ _ _ σ σ' _ => σ ⪯ σ');
     unfold assign, assign_new in *;
     repeat destruct_match;
     flatten; pM_trans ...
 Qed.
 Global Hint Resolve pM_theorem: pM.
 
-Theorem pM_theorem_list:
+Corollary pM_theorem_list:
   forall el σ σ' ρ ψ vl,
       ⟦_ el _⟧p (σ, ρ, ψ) --> (vl, σ') -> σ ⪯ σ'.
 Proof with (eauto with pM updates lia).
@@ -146,9 +118,9 @@ Proof with (eauto with pM updates lia).
 Qed.
 Global Hint Resolve pM_theorem_list: pM.
 
-Theorem pM_theorem_init:
-  forall fls ψ ρ σ σ',
-      initP fls ψ ρ σ σ' -> σ ⪯ σ'.
+Corollary pM_theorem_init:
+  forall C fls ψ ρ σ σ',
+      initP C fls ψ ρ σ σ' -> σ ⪯ σ'.
 Proof with (eauto with pM updates lia).
   intros.
   induction H;
@@ -157,58 +129,160 @@ Proof with (eauto with pM updates lia).
 Qed.
 Global Hint Resolve pM_theorem_init: pM.
 
-(** ** Other conservation results *)
-(** As a consequence, we have monotonicity on the sizes of stores *)
-Lemma evalP_dom:
-   forall e σ ρ ψ v σ',
-      ⟦e⟧p (σ, ρ, ψ) --> (v, σ') -> dom σ <= dom σ'.
-Proof.
-  eauto with pM.
-Qed.
-Global Hint Resolve evalP_dom: pM.
 
-Lemma evalListP_dom:
-   forall el σ ρ ψ vl σ',
-      ⟦_ el _⟧p (σ, ρ, ψ) --> (vl, σ') -> dom σ <= dom σ'.
-Proof.
-  eauto with pM.
-Qed.
-Global Hint Resolve evalListP_dom: pM.
+(** ** Exact monotonicity results *)
 
-Lemma initP_dom:
-  forall fls ψ ρ σ σ',
-      initP fls ψ ρ σ σ' -> dom σ <= dom σ'.
-Proof.
-  eauto with pM.
-Qed.
-Global Hint Resolve initP_dom: pM.
+(** ** Basic results on partial monotonicity*)
+(** The relation is trivially reflexive and transitive *)
+Lemma eM_refl: forall σ,
+    σ ⪳ σ.
+Proof. eauto with pM. Qed.
+Global Hint Resolve eM_refl: pM.
 
-Ltac eval_dom :=
+Lemma eM_trans : forall σ1 σ2 σ3,
+    σ1 ⪳ σ2 ->
+    σ2 ⪳ σ3 ->
+    σ1 ⪳ σ3.
+Proof.
+  unfold exact_monotonicity; intros.
+  specialize (H l C ω); steps.
+  specialize (H0 l C ω'); steps; eauto with pM lia.
+Qed.
+Global Hint Resolve eM_trans: pM.
+
+Ltac eM_trans :=
   repeat match goal with
-  | H: ⟦ ?e ⟧p (?σ, ?ρ, ?ψ) --> (?v, ?σ') |- _ =>
-    let fresh := fresh "H_dom" in
-    add_hypothesis fresh (evalP_dom e σ ρ ψ v σ' H)
-  | H: ⟦_ ?el _⟧p (?σ, ?ρ, ?ψ) --> (?vl, ?σ') |- _ =>
-    let fresh := fresh "H_dom" in
-    add_hypothesis fresh (evalListP_dom el σ ρ ψ vl σ' H)
-  | H: initP ?fls ?ψ ?ρ ?σ ?σ' |- _ =>
-    let fresh := fresh "H_dom" in
-    add_hypothesis fresh (initP_dom fls ψ ρ σ σ' H)
-  end.
+         | H:_ |- ?σ ⪳ ?σ => apply eM_refl
+         | H: ?σ1 ⪳ ?σ2 |- ?σ1 ⪳ ?σ3 => apply eM_trans with σ2 ; [ assumption | ]
+         | H: ?σ2 ⪳ ?σ3 |- ?σ1 ⪳ ?σ3 => apply eM_trans with σ2 ; [ | assumption ]
+         end.
+Global Hint Extern 1 => eM_trans: pM.
 
 
-(** If we combine partial monotonicity with compatibility (objects do no change type), we can prove that warm objects stay warm *)
-Lemma pM_warm_monotone:
+(** We have a result on the store sizes *)
+Lemma eM_domains:
+  forall σ σ',
+    σ ⪳ σ' -> dom σ <= dom σ'.
+Proof.
+  autounfold; unfold exact_monotonicity; intros.
+  destruct σ eqn:Σ; simpl; [lia |].
+  destruct o as [C ω].
+  specialize (H (dom s)).
+  destruct (getObj ((C, ω)::s) (dom s)) eqn: H__e.
+  - destruct o as [D ω'].
+    apply H in H__e; steps.
+    apply getObj_dom in H1; auto.
+  - unfold getObj in H__e.
+    apply nth_error_None in H__e.
+    simpl in H__e; lia.
+Qed.
+Global Hint Resolve eM_domains: pM.
+
+
+(** ** Main Monotonicity result *)
+(** We start with two technical results on partial monotonicity for assignment (update) and fresh location *)
+Lemma eM_assignment :
+  forall σ l C (ω ω': Env),
+    getObj σ l = Some (C, ω) ->
+    length ω = length ω' ->
+    σ ⪳ [l ↦ (C, ω')]σ.
+Proof.
+  autounfold with pM notations.
+  intros.
+  destruct_eq (l = l0); subst;
+    repeat rewrite_any;
+    rewrite getObj_update1 || rewrite getObj_update2;
+    eauto using getObj_dom.
+  steps. eexists; split; eauto.
+Qed.
+Global Hint Resolve eM_assignment: pM.
+
+Lemma eM_freshness :
+  forall σ c ρ,
+    σ ⪳ (σ ++ [(c, ρ)]).
+Proof.
+  autounfold with notations pM. unfold getObj; intros.
+  exists ω; steps.
+  rewrite nth_error_app1; eauto using getObj_dom.
+Qed.
+Global Hint Resolve eM_freshness: pM.
+
+(** Then we have the main result *)
+Theorem eM_theorem:
+  forall e σ σ' ρ ψ v,
+      ⟦e⟧ (σ, ρ, ψ) --> (v, σ') -> σ ⪳ σ'.
+Proof with (update_dom; eauto 3 with pM updates lia).
+  intros.
+  induction H using evalP_ind2 with
+    (Pl := fun _ σ _ _ _ σ' _ => σ ⪳ σ')
+    (Pin := fun C flds ψ _  σ σ' _ =>
+              forall ω Args Flds Mtds,
+                ct C = class Args Flds Mtds ->
+                getObj σ ψ = Some(C, ω) ->
+                dom ω + dom flds = dom Flds ->
+                σ ⪳ [ψ ↦ (C, repeat 0 (dom ω) )]σ');
+    unfold assign, assign_new in *;
+    repeat destruct_match; eval_dom;
+    flatten; pM_trans ...
+  - (* e_new *)
+    specialize (IHevalP0 [] _ _ _ H__ct (getObj_last _ _ _) ltac:(simpl;lia)).
+    lets: eM_domains IHevalP0...
+    intros l D ω H__get; steps.
+    lets [ω' [H__get1 ? ]] : IHevalP H__get; eauto.
+    lets : getObj_dom H__get1.
+    specialize (IHevalP0 l D ω' ltac:(rewrite getObj_last2; eauto using Lt.lt_le_trans with lia)) as [ω'' [ ]].
+    exists ω''; split ...
+    getObj_update; steps; try lia.
+  - intros. simpl in H1.
+    intros l; steps.
+    destruct_eq (l = I).
+    + exists (repeat 0 dom ω). subst.
+      rewrite getObj_update1 ...
+      rewrite H0 in H2; steps.
+      rewrite repeat_length. reflexivity.
+    + exists ω0.
+      rewrite getObj_update2...
+  - update_dom; steps.
+    intros l D ω' H__get; steps.
+    lets [ω'' [H__get1 ? ]] : IHevalP H3; eauto.
+    rewrite matched in H__get1; steps.
+    lets: getObj_dom matched.
+    lets: eM_domains IHevalP.
+    specialize (IHevalP0 (ω''++[v]) _ _ _ H2
+                         ltac: (eapply getObj_update1; eauto with lia)
+                                 ltac:(rewrite app_length; simpl; lia)).
+    lets [ω''' [ ]]: IHevalP l H__get.
+    destruct_eq (l = I); subst.
+    + rewrite H8 in matched; rewrite H__get in H3; steps.
+      exists (repeat 0 dom ω).
+      rewrite getObj_update1; try split ...
+      rewrite repeat_length. reflexivity.
+    + specialize (IHevalP0 l D ω''' ltac:(rewrite getObj_update2; eauto)) as [ω'''' [ ] ]...
+      exists ω''''.
+      getObj_update; steps; eauto; try lia.
+      rewrite getObj_update2 ...
+Qed.
+Global Hint Resolve eM_theorem: pM.
+
+Corollary eM_theorem_list:
+  forall el σ σ' ρ ψ vl,
+      ⟦_ el _⟧p (σ, ρ, ψ) --> (vl, σ') -> σ ⪳ σ'.
+Proof with (eauto with pM updates lia).
+  intros.
+  induction H ...
+Qed.
+Global Hint Resolve eM_theorem_list: pM.
+
+(** Exact monotonic stores keep objects warm *)
+From Celsius Require Import Reachability.
+Lemma eM_warm_monotone:
   forall σ σ' (l: Loc),
-    σ ⪯ σ' ->
-    σ ⪨ σ' ->
+    σ ⪳ σ' ->
     σ  ⊨ l : warm ->
     σ' ⊨ l : warm.
 Proof.
   autounfold with pM core notations. unfold reachable_warm.
   steps.
-  specialize (H l fields).
-  repeat rewrite_any.
-  eapply H0 in H2; steps.
+  lets [?ω' [ ] ] : H H1.
   repeat eexists; eauto.
 Qed.
