src/Semantics.v
@@ -2,8 +2,8 @@
 (* Clément Blaudeau - LAMP@EPFL 2021 *)
 (** This file defines the evaluator as a predicate and shows the equivalence with the functional version *)
 
-From Celsius Require Export Language Notations Helpers LibTactics.
-Require Import ssreflect ssrbool.
+From Celsius Require Export Language Notations Helpers LibTactics .
+Require Import ssreflect ssrbool  Coq.Program.Tactics.
 Import List Psatz Arith.
 Import ListNotations.
 Open Scope nat_scope.
@@ -22,19 +22,19 @@ Inductive evalP : Expr -> Store -> Env -> Value -> Value -> Store -> Prop :=
     getObj σ1 l1 = Some (C, f) ->
     getVal f x = Some v1 ->
     ⟦ (fld e0 x) ⟧p (σ, ρ, ψ) --> (v1, σ1)
-| e_mtd : forall σ e0 m el e2 ρ ψ l1 vl2 l3 σ1 σ2 σ3 C f argsC argsM fields methods T μ,
+| e_mtd : forall σ e0 m el e2 ρ ψ l1 vl2 l3 σ1 σ2 σ3 C Args Flds Mtds f argsM T μ,
     ⟦ e0 ⟧p (σ, ρ, ψ) --> (l1, σ1) ->
     getObj σ1 l1 = Some (C, f) ->
-    ct C = Some (class argsC fields methods) ->
-    methods m = Some (method μ argsM T e2) ->
+    ct C = class Args Flds Mtds  ->
+    Mtds m = Some (method μ argsM T e2) ->
     ⟦_ el _⟧p (σ1, ρ, ψ) --> (vl2, σ2) ->
     ⟦ e2 ⟧p (σ2, vl2, l1) --> (l3, σ3) ->
     ⟦ mtd e0 m el ⟧p (σ, ρ, ψ) --> (l3, σ3)
-| e_new : forall σ ρ ψ C args vl__args σ1 σ3 Tps Flds Mtds,
+| e_new : forall σ ρ ψ C Args Flds Mtds args vl__args σ1 σ3,
     ⟦_ args _⟧p (σ, ρ, ψ) --> (vl__args, σ1) ->
-    ct C = Some (class Tps Flds Mtds) ->
+    ct C = class Args Flds Mtds ->
     let I := (length σ1) in
-    initP Flds I vl__args (σ1 ++ [(C, [])]) σ3 ->
+    initP C Flds I vl__args (σ1 ++ [(C, [])]) σ3 ->
     ⟦ new C args ⟧p (σ, ρ, ψ) --> (I, σ3)
 | e_asgn : forall σ ρ ψ e1 x e2 e' σ1 v1 σ2 v2 σ3 v3,
     ⟦ e1 ⟧p (σ, ρ, ψ) --> (v1, σ1) ->
@@ -53,14 +53,14 @@ with evalListP : list Expr -> Store -> Env -> Value -> list Value -> Store -> Pr
     ⟦_ (e::el) _⟧p (σ, ρ, ψ) --> (l1::vl, σ2)
 where "'⟦_' el '_⟧p' '(' σ ',' ρ ',' v ')' '-->' '(' vl ',' σ0 ')' "  := (evalListP el σ ρ v vl σ0)
 
-with initP : list Field -> Var -> Env -> Store -> Store -> Prop :=
-| init_nil : forall I ρ σ,
-    initP [] I ρ σ σ
-| init_cons : forall I ρ σ v T e flds σ1 σ2 σ3,
+with initP : ClN -> list Field -> Var -> Env -> Store -> Store -> Prop :=
+| init_nil : forall C I ρ σ,
+    initP C [] I ρ σ σ
+| init_cons : forall C I ρ σ v T e flds σ1 σ2 σ3,
     ⟦ e ⟧p (σ, ρ, I) --> (v, σ1) ->
     assign_new I v σ1 = Some σ2 ->
-    initP flds I ρ σ2 σ3 ->
-    initP (field T e :: flds) I ρ σ σ3.
+    initP C flds I ρ σ2 σ3 ->
+    initP C (field T e :: flds) I ρ σ σ3.
 
 
 Global Instance notation_big_step_list_expr : notation_big_step (list Expr) (list Value) :=
@@ -72,7 +72,7 @@ Global Instance notation_big_step_expr : notation_big_step Expr Value :=
 Section evalP_ind.
   Variable P : forall e σ ρ ψ v σ', (evalP e σ ρ ψ v σ') -> Prop.
   Variable Pl : forall el σ ρ ψ vl σ', (evalListP el σ ρ ψ vl σ') -> Prop.
-  Variable Pin : forall flds ψ ρ σ σ', (initP flds ψ ρ σ σ') -> Prop.
+  Variable Pin : forall C flds ψ ρ σ σ', (initP C flds ψ ρ σ σ') -> Prop.
 
   Variable P_var : forall σ x ρ ψ l Hget,
       P (var x) σ ρ ψ l σ (e_var σ x ρ ψ l Hget).
@@ -90,10 +90,10 @@ Section evalP_ind.
     P e2 σ2 vl2 v1 v3 σ3 H__e2 ->
     P( mtd e0 m el) σ ρ ψ v3 σ3 (e_mtd σ e0 m el e2 ρ ψ v1 vl2 v3 σ1 σ2 σ3 C f argsC argsM fields methods T μ H__e0 Hobj Hct Hmth H__el H__e2).
 
-  Variable P_new : forall σ ρ ψ C args vl__args σ1 σ3 Tps Flds Mtds H__args H__ct H__init,
+  Variable P_new : forall σ ρ ψ C args vl__args σ1 σ3 Args Flds Mtds H__args H__ct H__init,
     Pl args σ ρ ψ vl__args σ1 H__args ->
-    Pin Flds (length σ1) vl__args (σ1 ++ [(C, [])]) σ3 H__init ->
-    P (new C args) σ ρ ψ (length σ1) σ3 (e_new σ ρ ψ C args vl__args σ1 σ3 Tps Flds Mtds H__args H__ct H__init).
+    Pin C Flds (length σ1) vl__args (σ1 ++ [(C, [])]) σ3 H__init ->
+    P (new C args) σ ρ ψ (length σ1) σ3 (e_new σ ρ ψ C Args Flds Mtds args vl__args σ1 σ3 H__args H__ct H__init).
 
   Variable P_asgn :  forall σ ρ ψ e1 x e2 e' σ1 v1 σ2 v2 σ3 v3 H__e1 H__e2 H__e',
     P e1 σ ρ ψ v1 σ1 H__e1 ->
@@ -108,14 +108,12 @@ Section evalP_ind.
       Pl el σ1 ρ ψ vl σ2 H__el ->
       Pl (e::el) σ ρ ψ (v1::vl) σ2 (el_cons σ ρ ψ e el v1 σ1 vl σ2 H__e H__el).
 
-  Variable Pin_nil: forall I (ρ: Env) (σ: Store), Pin [] I ρ σ σ (init_nil I ρ σ).
+  Variable Pin_nil: forall C I ρ σ, Pin C [] I ρ σ σ (init_nil C I ρ σ).
 
-  Variable Pin_cons : forall I ρ σ v T e flds σ1 σ2 σ3 H__e H__assign H__flds,
+  Variable Pin_cons : forall C I ρ σ v T e flds σ1 σ2 σ3 H__e H__assign H__flds,
       P e σ ρ I v σ1 H__e ->
-      Pin flds I ρ σ2 σ3 H__flds ->
-      Pin (field T e :: flds) I ρ σ σ3 (init_cons I ρ σ v T e flds σ1 σ2 σ3 H__e H__assign H__flds).
-
-  Variable Pin_magic : forall flds ψ ρ σ σ' H__init, Pin flds ψ ρ σ σ' H__init.
+      Pin C flds I ρ σ2 σ3 H__flds ->
+      Pin C (field T e :: flds) I ρ σ σ3 (init_cons C I ρ σ v T e flds σ1 σ2 σ3 H__e H__assign H__flds).
 
   Fixpoint evalP_ind2 e σ ρ ψ v σ' (eval : evalP e σ ρ ψ v σ') : P e σ ρ ψ v σ' eval :=
     match eval with
@@ -128,10 +126,10 @@ Section evalP_ind.
               (evalP_ind2 e0 σ ρ ψ l1 σ1 H__e0)
               (evalListP_ind2 el σ1 ρ ψ vl2 σ2 H__el)
               (evalP_ind2 e2 σ2 vl2 l1 l3 σ3 H__e2)
-    | e_new σ ρ ψ C args vl__args σ1 σ3 Tps Flds Mtds H__args H__ct H__init =>
-        P_new σ ρ ψ C args vl__args σ1 σ3 Tps Flds Mtds H__args H__ct H__init
+    | e_new σ ρ ψ C Args Flds Mtds args vl__args σ1 σ3 H__args H__ct H__init =>
+        P_new σ ρ ψ C args vl__args σ1 σ3 Args Flds Mtds H__args H__ct H__init
               (evalListP_ind2 args σ ρ ψ vl__args σ1 H__args)
-              (initP_ind2 Flds (length σ1) vl__args (σ1 ++ [(C, [])]) σ3 H__init )
+              (initP_ind2 C Flds (length σ1) vl__args (σ1 ++ [(C, [])]) σ3 H__init)
     | e_asgn σ ρ ψ e1 x e2 e' σ1 v1 σ2 v2 σ3 v3 H__e1 H__e2 H__e' =>
         P_asgn σ ρ ψ e1 x e2 e' σ1 v1 σ2 v2 σ3 v3 H__e1 H__e2 H__e'
                (evalP_ind2 e1 σ ρ ψ v1 σ1 H__e1)
@@ -148,14 +146,66 @@ Section evalP_ind.
                      (evalListP_ind2 el σ1 ρ ψ vl σ2 H__el)
          end
 
-  with initP_ind2 flds ψ (ρ:Env) (σ σ':Store) H__init : Pin flds ψ ρ σ σ' H__init :=
+  with initP_ind2 C flds ψ (ρ:Env) (σ σ':Store) H__init: Pin C flds ψ ρ σ σ' H__init :=
          match H__init with
-         | init_nil ψ ρ σ => Pin_nil ψ ρ σ
-         | init_cons ψ ρ σ v T e flds σ1 σ2 σ3 H__e H__assign H__flds =>
-                       Pin_cons ψ ρ σ v T e flds σ1 σ2 σ3 H__e H__assign H__flds
-                                (evalP_ind2 e σ ρ ψ v σ1 H__e)
-                                (initP_ind2 flds ψ ρ σ2 σ3 H__flds)
+         | init_nil C ψ ρ σ => Pin_nil C ψ ρ σ
+         | init_cons C ψ ρ σ v T e flds σ1 σ2 σ3 H__e H__assign H__flds =>
+             Pin_cons C ψ ρ σ v T e flds σ1 σ2 σ3 H__e H__assign H__flds
+                      (evalP_ind2 e σ ρ ψ v σ1 H__e)
+                      (initP_ind2 C flds ψ ρ σ2 σ3 H__flds)
          end.
 
 
 End evalP_ind.
+
+
+(** ** Conservation result *)
+(** The monotonicity on the size of the store is easy to obtain via induction *)
+Theorem evalP_dom:
+  forall e σ ρ ψ v σ',
+      ⟦e⟧ (σ, ρ, ψ) --> (v, σ') -> dom σ <= dom σ'.
+Proof with (eauto with updates lia).
+  intros.
+  induction H using evalP_ind2 with
+    (Pl := fun _ σ _ _ _ σ' _ => dom σ <= dom σ')
+    (Pin := fun _ _ _ _ σ σ' _ => dom σ <= dom σ');
+    unfold assign, assign_new in *; steps;
+    update_dom;
+    repeat rewrite_anywhere app_length; simpl in * ...
+Qed.
+
+Corollary evalListP_dom:
+   forall el σ ρ ψ vl σ',
+      ⟦_ el _⟧p (σ, ρ, ψ) --> (vl, σ') -> dom σ <= dom σ'.
+Proof with (try lia).
+  intros.
+  induction H ...
+  eapply evalP_dom in H ...
+Qed.
+Global Hint Resolve evalListP_dom: pM.
+
+Corollary initP_dom:
+  forall C fls ψ ρ σ σ',
+      initP C fls ψ ρ σ σ' -> dom σ <= dom σ'.
+Proof with (try lia).
+  intros.
+  induction H ...
+  eapply evalP_dom in H ...
+  unfold assign_new in *; ground;
+    update_dom;
+    eauto with lia updates ...
+Qed.
+Global Hint Resolve initP_dom: pM.
+
+Ltac eval_dom :=
+  repeat match goal with
+  | H: ⟦ ?e ⟧p (?σ, ?ρ, ?ψ) --> (?v, ?σ') |- _ =>
+    let fresh := fresh "H_dom" in
+    add_hypothesis fresh (evalP_dom e σ ρ ψ v σ' H)
+  | H: ⟦_ ?el _⟧p (?σ, ?ρ, ?ψ) --> (?vl, ?σ') |- _ =>
+    let fresh := fresh "H_dom" in
+    add_hypothesis fresh (evalListP_dom el σ ρ ψ vl σ' H)
+  | H: initP ?C ?fls ?ψ ?ρ ?σ ?σ' |- _ =>
+    let fresh := fresh "H_dom" in
+    add_hypothesis fresh (initP_dom C fls ψ ρ σ σ' H)
+  end.
