src/Wellformedness.v
@@ -2,187 +2,82 @@
 (* Clément Blaudeau - Lamp@EPFL 2021 *)
 (** This file defines the notion of wellformedness for scopes. The set of reachable locations must all be valid locations of the store - that is, locations that are inside of the store. The main result is to show that if we start from a wellformed store that contains the local environment ρ and the [this] pointer, then we end up with a wellformed store that contains the location of the result *)
 
-From Celsius Require Export PartialMonotonicity Reachability Compatibility.
-Require Import ssreflect ssrbool Psatz List Sets.Ensembles Coq.Program.Tactics.
+From Celsius Require Export Reachability Semantics PartialMonotonicity.
+Require Import ssreflect ssrbool Psatz List Sets.Ensembles Coq.Program.Tactics Coq.Sets.Finite_sets_facts.
 Import ListNotations.
 Open Scope nat_scope.
-
-Global Hint Resolve Union_intror: wf.
-Global Hint Resolve Union_introl: wf.
-Global Hint Resolve In_singleton: wf.
 
 (** ** Definitions and notations *)
 (** A wellformed store only contains pointers to locations that are within itself *)
 Definition wf σ :=
   forall l C ω,
-    getObj σ l = Some(C,ω) ->
-    forall f l,
-      getVal ω f = Some l ->
-      l < dom σ. (**r [l ∈ dom σ] *)
+    getObj σ l = Some(C, ω) ->
+    (forall Args Flds Mtds,
+        ct C = class Args Flds Mtds ->
+        dom ω <= dom Flds) /\
+      (forall f l',
+          getVal ω f = Some l' ->
+          l' < dom σ).
 
-(** A set of locations is contained in a store: [L ⪽ σ] *)
-Definition storeSubset (σ: Store) L :=
-  forall l, l ∈ L ->
-       l < dom σ.
-
-(** The codomain of an environment is the set of locations it contains *)
-Definition codom (ρ: Env) : (LocSet) :=
-  fun l => (List.In l ρ).
-
-Notation "L ⪽ σ" := (storeSubset σ L) (at level 80).
-Notation " a ∪ { b } " := (Union Loc a (Singleton Loc b)) (at level 80).
-
-(** ** Basic results *)
-
-Lemma storeSubset_trans :
-  forall a s s',
-    dom s <= dom s' ->
-    a ⪽ s ->
-    a ⪽ s'.
-Proof.
-  unfold storeSubset; steps.
-  eapply H0 in H1 ; lia.
-Qed.
-
-Lemma storeSubset_union :
-  forall a b s,
-    a ⪽ s ->
-    b ⪽ s ->
-    (a∪b) ⪽ s.
-Proof.
-  unfold storeSubset; intros.
-  induction H1; eauto.
-Qed.
-
-Lemma storeSubset_union_l :
-  forall a b s,
-    (a∪b) ⪽ s -> a ⪽ s.
-Proof.
-  unfold storeSubset; eauto with wf.
-Qed.
-
-Lemma storeSubset_union_r :
-  forall a b s,
-    (a∪b) ⪽ s -> b ⪽ s.
-Proof.
-  unfold storeSubset; eauto with wf.
-Qed.
-
-Lemma storeSubset_add :
-  forall v a s,
-    codom (v :: a) ⪽ s <-> v < dom s /\ codom a ⪽ s.
-Proof.
-  unfold codom, List.In, In, storeSubset in *; split.
-  + steps; eapply_any; steps; right => //.
-  + steps; move: H0 => [Hl|Hl]; steps.
-Qed.
-
-Lemma storeSubset_singleton :
-  forall a b σ,
-    a ∪ {b} ⪽ σ -> b < dom σ.
+Lemma wf_proj1 : forall σ l C ω f v,
+    wf σ ->
+    getObj σ l = Some (C, ω) ->
+    getVal ω f = Some v ->
+    v < dom σ.
 Proof.
   intros.
-  eapply_any; eauto with wf.
+  eapply H; eauto.
 Qed.
+Global Hint Resolve wf_proj1: wf.
 
-Lemma storeSubset_singleton2 :
-  forall a σ,
-    (Singleton Loc a) ⪽ σ -> a < dom σ.
-Proof.
-  unfold storeSubset; steps.
-  induction (H a) ; steps.
-Qed.
-
-Lemma storeSubset_singleton3 :
-  forall a σ,
-    a < dom σ -> (Singleton Loc a) ⪽ σ.
-Proof.
-  unfold storeSubset; steps;
-    induction H0 ; steps.
-Qed.
-
-Lemma storeSubset_codom_empty : forall s, codom [] ⪽ s.
-Proof.
-  unfold storeSubset; steps.
-Qed.
-
-Lemma codom_empty_union: forall a, (codom [] ∪ a) = a.
+Lemma wf_proj2 : forall σ l C ω Args Flds Mtds,
+    wf σ ->
+    getObj σ l = Some (C, ω) ->
+    ct C = class Args Flds Mtds ->
+    dom ω <= dom Flds.
 Proof.
   intros.
-  apply Extensionality_Ensembles.
-  unfold Same_set, Included;
-    repeat steps || destruct H;
-    eauto with wf.
+  eapply H; eauto.
 Qed.
-
-Lemma codom_cons:
-  forall a ρ, codom (a::ρ) = ({a} ∪ (codom ρ)).
-Proof.
-  intros; apply Extensionality_Ensembles.
-  unfold Same_set; steps; intros l; steps; try inversion H; steps;
-    try inSingleton;
-    eauto using Union_introl, Union_intror.
-Qed.
-
-
-Lemma storeSubset_update:
-  forall L l o σ,
-    L ⪽ [l ↦ o] (σ) -> L ⪽ σ.
-Proof.
-  unfold storeSubset; steps; update_dom; eauto.
-Qed.
-Global Hint Resolve storeSubset_update: wf.
+Global Hint Resolve wf_proj2: wf.
 
 
 (** In preparation for initialization theorems, we have technical results about adding a location *)
-Lemma wf_add : forall s c ρ, wf s -> codom ρ ⪽ s -> wf (s ++ [(c,ρ)]).
-Proof.
-  unfold wf; intros.
+Lemma wf_add : forall s C ρ Args Flds Mtds,
+    wf s ->
+    codom ρ ⪽ s ->
+    ct C = class Args Flds Mtds ->
+    dom ρ <= dom Flds ->
+    wf (s ++ [(C,ρ)]).
+Proof with (eauto with wf lia).
+  steps.
+  unfold wf; simpl; intros.
   rewrite app_length; simpl.
   destruct_eq (l = length s);
-    [subst; rewrite_anywhere getObj_last | rewrite_anywhere getObj_last2]; eauto.
-  + invert_constructor_equalities; subst.
-    apply PeanoNat.Nat.lt_trans with (length s); [| lia].
-    eapply H0, nth_error_In, H2.
-  + apply PeanoNat.Nat.lt_trans with (length s); [| lia]; eauto.
-  + apply getObj_dom in H1.
+    [subst; try rewrite_anywhere getObj_last | try rewrite_anywhere getObj_last2].
+  + steps.
+    specialize (H0 l') as [ ] ...
+  + split; intros...
+    lets [ _ ? ]: H H3 ...
+    lets : H5 H4 ...
+  + apply getObj_dom in H3.
     rewrite_anywhere  app_length; simpl in *.
     assert (l < length s) by lia ; eauto.
 Qed.
+Global Hint Resolve wf_add: wf.
 
-Lemma wf_add_empty : forall s c, wf s -> wf (s ++ [(c,[])]).
-Proof.
-  eauto using wf_add, storeSubset_codom_empty.
-Qed.
-
-Lemma getVal_codom : forall x l ρ,
-    getVal ρ x = Some l -> l ∈ codom ρ.
+Lemma wf_add_empty : forall s C,
+    wf s ->
+    wf (s ++ [(C,[])]).
 Proof.
   intros.
-  eapply nth_error_In in H. auto.
+  destruct (ct C) eqn:H__ct.
+  eapply wf_add; eauto using storeSubset_codom_empty with cbn lia.
 Qed.
-
-
-(** We add all hints *)
-Global Hint Resolve storeSubset_trans: wf.
-Global Hint Resolve storeSubset_union: wf.
-Global Hint Resolve storeSubset_union_l: wf.
-Global Hint Resolve storeSubset_add: wf.
-Global Hint Resolve storeSubset_union_r: wf.
-Global Hint Resolve storeSubset_singleton: wf.
-Global Hint Resolve storeSubset_singleton2: wf.
-Global Hint Resolve storeSubset_singleton3: wf.
-Global Hint Resolve storeSubset_codom_empty: wf.
-Global Hint Resolve wf_add: wf.
 Global Hint Resolve wf_add_empty: wf.
-Global Hint Resolve nth_error_In: wf.
-Global Hint Resolve storeSubset_update: wf.
-Global Hint Resolve getVal_codom: wf.
-Global Hint Rewrite codom_cons: wf.
+
 
 (** ** Evaluation-maintained results *)
-(** We want to show that the evaluator maintains the wellformedness of stores. As it is not only about stores but also the location of [this] and the result, we cannot use the results proved in Eval.v. We reprove it from scratch, starting with some technical results. *)
-
 (** First a technical result on assignment *)
 Lemma wf_assign:
   forall σ ω l v f C,
@@ -191,68 +86,94 @@ Lemma wf_assign:
     wf σ ->
     wf [l ↦ (C, [f ↦ v]ω)]σ .
 Proof.
-  unfold wf; steps.
+  unfold wf; intros.
   rewrite update_dom.
-  getObj_update; steps; eauto.
+  getObj_update.
+  destruct H2; steps;
+    try rewrite update_one3; steps;
+    try solve [eapply H1; eauto].
   getVal_update; steps; eauto.
+  eapply H1; eauto.
 Qed.
 Global Hint Resolve wf_assign: wf.
-
 Global Hint Unfold storeSubset: wf.
+
+Ltac cross_rewrites :=
+  repeat match goal with
+         | H: ?A = ?B, H': ?A = ?C |- _ => rewrite H in H'; inverts H'
+         end.
+
 
 (** Then we have the main result *)
 Theorem wf_theorem :
-  forall e σ ρ ψ v σ',
-    ⟦e⟧p (σ, ρ, ψ) --> (v, σ') ->
+ forall e σ ρ ψ v σ',
+    ⟦e⟧ (σ, ρ, ψ) --> (v, σ') ->
     wf σ ->
     (codom ρ) ∪ {ψ} ⪽ σ ->
     (wf σ' /\ v < dom σ').
-Proof with (eauto with wf lia).
-  intros. move: H0 H1.
+Proof with (update_dom; eauto with wf pM updates lia).
+  intros.
+  move: H0 H1.
   induction H using evalP_ind2 with
     (Pl := fun _ σ ρ ψ vl σ' _ => (codom ρ ∪ {ψ}) ⪽ σ -> wf σ -> (wf σ' /\ codom vl ⪽ σ'))
-    (Pin := fun _ ψ ρ σ σ' _   => (codom ρ ∪ {ψ}) ⪽ σ -> wf σ -> wf σ');
+    (Pin := fun C flds ψ ρ σ σ' _ =>
+              forall (H__codom : codom ρ ∪ {ψ} ⪽ σ) (H__wf: wf σ) ω Args Flds Mtds
+                (H__ct : ct C = class Args Flds Mtds) (H__obj: getObj σ ψ = Some(C, ω)),
+                dom ω + dom flds = dom Flds ->
+                 (exists ω', getObj σ' ψ = Some (C, ω') /\ dom ω' = dom Flds) /\ wf σ');
     unfold assign, assign_new in * ; intros; eval_dom ...
+  - (* e_var *)
+    intuition auto ...
   - (* e_fld *)
-    steps. eapply_any ...
-  - (* e_mtd *)
-    destruct IHevalP3, IHevalP2; steps ...
+    destruct IHevalP1...
+    destruct IHevalP2...
   - (* e_new *)
     destruct IHevalP ...
-    rewrite dom_app in H2.
-    steps ...
-    eapply IHevalP0 ...
-    eapply storeSubset_union;
+    edestruct IHevalP0; eauto with lia wf.
+    + eapply storeSubset_union;
       [ eapply storeSubset_trans with σ1 |
         eapply storeSubset_singleton3] ; try rewrite dom_app ...
+    + rewrite getObj_last ...
+    + reflexivity.
   - (* e_assgn *)
     destruct IHevalP1 ...
     destruct IHevalP2 ...
     repeat destruct_match; subst;
       destruct IHevalP3 ...
-    eapply storeSubset_trans with σ ...
-    rewrite update_dom ...
   - (* el_cons *)
     destruct IHevalP ...
-    destruct IHevalP0 ...
-    steps. apply storeSubset_add...
+    destruct IHevalP0; steps ...
+    apply storeSubset_add...
+  - (* init_nil *)
+    simpl in *.
+    split; [eexists; split |] ...
   - (* init_cons *)
     destruct IHevalP ...
-    destruct (getObj σ1 I) eqn:H__obj; steps ;
+    destruct (getObj σ1 I) as [[?C ?ω] |] eqn:?H__obj;
       repeat rewrite_anywhere update_dom ...
-    eapply IHevalP0 ...
+    invert_constructor_equalities; subst. update_dom.
+    simpl in H0.
+    lets [?ω [ ] ]: eM_theorem H H__obj. cross_rewrites.
+    edestruct IHevalP0; eauto.
     + eapply storeSubset_trans with σ ...
-      rewrite update_dom ...
-    + intros l; intros.
-      getObj_update; steps; try rewrite update_dom; try lia.
-      * eapply getVal_add in H7; steps ...
-        eapply H4 ...
-      * eapply H4 ...
+    + intros l ?C ?ω ?H__obj; update_dom.
+      destruct_eq (l = I); subst.
+      * rewrite getObj_update1 in H__obj1. apply getObj_dom in H__obj ...
+        invert_constructor_equalities; subst.
+        pose proof H__obj0.
+        split.
+        -- intros; cross_rewrites. rewrite app_length; simpl ...
+        -- intros.
+           apply getVal_add in H7; steps ...
+           eapply wf_proj1 ...
+      * rewrite getObj_update2 in H__obj1; eauto. apply getObj_dom in H__obj ...
+    + rewrite getObj_update1 ...
+    + rewrite app_length; simpl ...
 Qed.
 
-Theorem wf_theorem_list :
-  forall el σ ρ ψ vl σ',
-    ⟦_ el _⟧p (σ, ρ, ψ) --> (vl, σ') ->
+Corollary wf_theorem_list :
+  forall (el: list Expr) σ ρ ψ vl σ',
+    ⟦ el ⟧ (σ, ρ, ψ) --> (vl, σ') ->
     (codom ρ ∪ {ψ}) ⪽ σ ->
     wf σ ->
     wf σ' /\ (codom vl ⪽ σ').
@@ -267,6 +188,44 @@ Proof with (eauto with wf lia).
     apply IHevalListP ...
 Qed.
 Global Hint Resolve wf_theorem_list: wf.
+
+Corollary wf_theorem_init :
+  forall C flds ψ ρ σ σ' Args Flds Mtds ω,
+    initP C flds ψ ρ σ σ' ->
+    codom ρ ∪ {ψ} ⪽ σ ->
+    wf σ ->
+    ct C = class Args Flds Mtds ->
+    getObj σ ψ = Some(C, ω) ->
+    dom ω + dom flds = dom Flds ->
+    (exists ω', getObj σ' ψ = Some (C, ω') /\ dom ω' = dom Flds) /\ wf σ'.
+Proof with (update_dom; eauto with wf lia).
+  intros. move: H0 H1 H2 H3 H4. gen ω.
+  induction H; intros; eval_dom ...
+  - steps ...
+  - simpl in *.
+    lets [ ] : wf_theorem H; eauto.
+    unfold assign_new in *.
+    destruct (getObj σ1 I) as [[?C ?ω] |] eqn:?H__obj; update_dom ...
+    invert_constructor_equalities; subst ...
+    lets [?ω [ ] ]: eM_theorem H H5. cross_rewrites.
+    eapply IHinitP ...
+    + eapply storeSubset_trans with σ ...
+    + intros l ?C ?ω ?H__obj; update_dom.
+      destruct_eq (l = I); subst.
+      * rewrite getObj_update1 in H__obj0. apply getObj_dom in H5 ...
+        invert_constructor_equalities; subst.
+        pose proof H__obj.
+        split.
+        -- intros; cross_rewrites. rewrite app_length; simpl ...
+        -- intros.
+           apply getVal_add in H12; steps ...
+           eapply wf_proj1 ...
+      * rewrite getObj_update2 in H__obj0; eauto. apply getObj_dom in H__obj ...
+    + rewrite getObj_update1 ...
+    + rewrite app_length; simpl ...
+Qed.
+Global Hint Resolve wf_theorem_list: wf.
+
 
 (* A simple corollary on the conservation of wellformedness *)
 Corollary wf_conserved :
@@ -318,3 +277,19 @@ Ltac eval_wf :=
               eauto with wf pM
           end
   end.
+
+(** Partially monotonic wellformed stores keep objects warm *)
+Lemma pM_wf_warm_monotone:
+  forall σ σ' (l: Loc),
+    σ ⪯ σ' ->
+    wf σ' ->
+    σ  ⊨ l : warm ->
+    σ' ⊨ l : warm.
+Proof.
+  autounfold with pM core notations. unfold reachable_warm.
+  steps.
+  lets [?ω' [ ] ] : H H2.
+  lets [ ? _ ]: H0 H3.
+  lets : H6 H1.
+  repeat eexists; eauto with lia.
+Qed.
