src/LocalReasoning.v
@@ -2,7 +2,7 @@
 (* Clément Blaudeau - Lamp@EPFL 2021 *)
 (** This file defines the main result of local reasoning, built upon wellformedness, compatibility, scopability and stackability. In a wellformed, fully initialized context, a newly created object can only access hot (transitively fully initialized) locations. *)
 
-From Celsius Require Export Scopability Compatibility PartialMonotonicity Stackability MetaTheory.
+From Celsius Require Export Scopability PartialMonotonicity Stackability MetaTheory.
 Require Import ssreflect ssrbool Psatz Sets.Ensembles List Coq.Sets.Finite_sets_facts.
 Import ListNotations.
 Open Scope nat_scope.
@@ -13,9 +13,9 @@ Lemma local_reasoning:
   forall (σ σ': Store) (L L': LocSet),
     L ⪽ σ ->
     L' ⪽ σ' ->
+    wf σ' ->
     (σ, L) ⋖ (σ', L') ->
     σ ≪ σ' ->
-    σ ⪨ σ' ->
     σ ⪯ σ' ->
     σ  ⊨ L  : hot ->
     σ' ⊨ L' : hot.
@@ -25,15 +25,15 @@ Proof.
   assert (dom σ <= dom σ') by eauto with pM.
   destruct (PeanoNat.Nat.lt_ge_cases l (dom σ)).
   + (* l ∈ (dom σ) : the object was already in the store *)
-    eapply pM_warm_monotone; eauto.
+    eapply pM_wf_warm_monotone; eauto.
     assert (σ ⊨ L ⇝ l).
-    * eapply H1 ; simpl => //.
+    * eapply H2 ; simpl => //.
       exists l'; split; eauto with rch.
     * rch_set.
       eapply H5; eauto with rch.
   + (* l ∉ (dom σ) *)
     pose proof (reachability_dom _ _ _ H6).
-    destruct (H2 l); eauto with lia.
+    destruct (H3 l); eauto with lia.
 Qed.
 
 (* Then the main theorem : *)
@@ -48,7 +48,7 @@ Proof.
   intros.
   assert (σ' ⊨ (Singleton Loc v) : hot).
   + eapply local_reasoning;
-      eauto using stk_theorem with pM stk cmpt wf lia.
+      eauto using stk_theorem with pM stk wf lia.
     eapply scopability_theorem in H; eauto with pM wf lia; steps.
   + eapply H3; eauto using In_singleton.
 Qed.
@@ -85,7 +85,7 @@ Lemma synchronization: forall Σ σ (l: Loc),
         Σ ▷ Σ' /\
         Σ ≪ Σ' /\
         (forall (l': Loc), σ ⊨ l ⇝ l' -> Σ' ⊨ l' : hot).
-Proof with (meta; eauto with typ).
+Proof with (meta; eauto with typ updates lia).
   intros Σ σ l H__wf H__st; intros.
   remember ((fun l' '(C,μ) => if (reachabilityb σ l l') then (C, hot) else (C, μ)):Loc -> Tpe -> Tpe) as f.
   remember (map (fun '(l, T) => (l, f l T)) Σ) as Σ'.
@@ -103,13 +103,24 @@ Proof with (meta; eauto with typ).
         erewrite getType_map; steps; eauto.
         inverts matched. reflexivity.
       * inverts H4; meta; eauto with typ.
-        apply ot_hot; intros f v H__val.
-        assert (σ ⊨ l ⇝ v) by eauto with rch.
+        destruct (ct C0) as [Args Flds Mtds] eqn:?.
+        eapply ot_hot...
+        intros f ?C ?μ. intros.
+        assert (f < dom ω). {
+          inverts H3;
+            inverts H2 ...
+          - lets : H9 H1 H4; steps ...
+          - lets : H9 H1 H4; steps ...
+        }
+        destruct (getVal ω f) eqn:?H__val ; [| apply nth_error_None in H__val; lia]...
+        exists v; split => //.
+        assert (σ ⊨ l ⇝ v) by eauto with rch wf.
         assert (Σ ⊨ v : warm) by eauto.
-        inverts H4. inverts H6 ...
-        exists x, (x, hot) ...
-        erewrite getType_map ...
+        exists (C, hot) ...
+        erewrite getType_map ... step...
         destruct (reachability_refl σ l v); steps.
+        assert (C1 = C); eauto.
+        invert H3; inverts H2; eauto; try lets [?v [ ] ]: H15 H4...
     + exists C, ω, μ; repeat split => // ...
       erewrite getType_map ...
       destruct (reachability_refl σ l l'); steps.
@@ -150,36 +161,40 @@ Lemma local_reasoning2: forall Σ1 Σ2 σ1 σ2 (L1 L2: LocSet),
     (Σ1 ⊨ σ1) ->
     (Σ2 ⊨ σ2) ->
     (Σ1 ⊨ L1 : hot) ->
+    wf σ1 ->
     wf σ2 ->
-    exists Σ', (Σ1 ≪ Σ') /\
-            (Σ1 ≼ Σ') /\
-            (Σ1 ▷ Σ') /\
+    (forall l2, l2 ∈ L2 -> in_dom Σ2 l2) ->
+    exists Σ', (Σ2 ≪ Σ') /\
+            (Σ2 ≼ Σ') /\
+            (Σ2 ▷ Σ') /\
             (Σ' ⊨ σ2) /\
             (Σ' ⊨ L2 : hot).
-Proof.
+Proof with (meta; eauto with typ lia).
   intros Σ1 Σ2 σ1 σ2 L1 L2 H1 H2.
   pose proof (storeSubset_finite _ _ H2).
   gen Σ1 Σ2 σ1 σ2 L1.
   eapply finite_sets_ind with (F := L2); eauto; intros.
-  - exists Σ2; steps.
+  - exists Σ2; steps ...
     intros l Hl. inversion Hl.
-  - clear H L2. rename F into L2, a into l2.
+  - clear H L2. rename F into L2, a into l, H13 into H_in.
     unfold Add in *.
     assert ((σ1, L1) ⋖ (σ2, L2)) by eauto with scp.
     pose proof (storeSubset_union_l _ _ _ H2).
-    specialize (H1 Σ1 Σ2 σ1 σ2 H12 L1 H3 H H5 H6 H7 H8 H9 H10) as [Σ2' [ ]]; steps.
-    clear Σ2 H5 H6 H7 H9.
-    pose proof (synchronization Σ2' σ2 l2 H11 H15) as [Σ'' [ ]] ; steps.
+    lets [Σ3 [ ]]: H1 Σ2 H10; eauto; steps. apply H_in; eauto with wf.
+    assert (H_in':forall l2 : Loc, l2 ∈ (L2 ∪ {l}) -> in_dom Σ3 l2) ...
+    (* clear Σ1 H5 H6 H7 H8 H10 H1. *) clear H1.
+    lets [Σ4 [ ]]: synchronization Σ3 σ2 l H17; steps...
     + assert (l' < dom σ1 \/ l' >= dom σ1) as [|] by lia.
-      * specialize (H4 H3 H2 l' H6) as[l1 [H__l1 H__rch1]];[ exists l2; split; eauto with wf |].
-        specialize (H10 l1 H__l1).
-        lets: hot_transitivity  H10 H8 H__rch1.
-        specialize (H14 l').
-        meta; steps; meta; eauto with typ.
-        exists C. eapply vt_sub; eauto with typ.
-      * specialize (H1 l') as [ ]; eauto.
-        -- assert (in_dom Σ2' l2) by admit.
-        -- specialize (H8 l' H1); steps. apply getObj_dom in H8. lia.
-    + exists Σ''; repeat split; eauto with typ.
+      * lets [l1 [H__l1 H__rch1]] : H4 H3 H2 l' H18; [ exists l; split; eauto with wf |].
+        lets : H10 H__l1.  clear H10.
+        lets: hot_transitivity H20 H__rch1...
+        lets: mn_trans H7 H16.
+        specialize (H22 l' H10) as [?T1 [?T2 [? [ ]]]] ...
+        exists C, (C,hot)...
+      * lets: stk_st_trans H5 H14 H16.
+        specialize (H20 l') as [ ]; eauto.
+        -- admit.
+        -- specialize (H8 l' H20); steps ... apply getObj_dom in H21. lia.
+    + exists Σ4; repeat split; eauto with typ.
       intros l0 [ l2' | ]; try inSingleton; eauto with rch wf typ.
-Qed.
+Admitted.
